src/Parsers/BooleanRecognizerExt.v
@@ -1,0 +1,324 @@
+(** * Extensionality of boolean recognizer *)
+Require Import Fiat.Parsers.ContextFreeGrammar.Core.
+Require Import Fiat.Parsers.BaseTypes.
+Require Import Fiat.Parsers.StringLike.Core.
+Require Import Fiat.Parsers.StringLike.Properties.
+Require Import Fiat.Parsers.BooleanRecognizer.
+Require Import Fiat.Common.
+Require Import Fiat.Common.Equality.
+Require Import Fiat.Common.List.ListMorphisms.
+(*Require Import Coq.Lists.List.
+Require Import Coq.Arith.EqNat.
+Require Import Coq.Arith.Compare_dec Coq.Arith.Wf_nat.
+Require Import Coq.omega.Omega.
+Require Import Fiat.Common.List.Operations.
+Require Import Fiat.Parsers.ContextFreeGrammar.
+Require Import Fiat.Parsers.BaseTypes.
+Require Import Fiat.Parsers.StringLike.Properties.
+Require Import Fiat.Common Fiat.Common.Wf.*)
+
+Set Implicit Arguments.
+Local Open Scope string_like_scope.
+
+Section recursive_descent_parser.
+  Context {Char} {HSL : StringLike Char} {G : grammar Char}.
+  Context {data : @boolean_parser_dataT Char _}.
+
+  Create HintDb boolr_ext_db discriminated.
+  Hint Unfold Proper respectful respectful_hetero pointwise_relation forall_relation pointwise2_relation sumbool_rect : boolr_ext_db.
+
+  Local Ltac expand' :=
+    idtac;
+    (lazymatch goal with
+    | [ |- ?R = ?L ]
+      => (let rh := head R in
+          let lh := head L in
+          constr_eq rh lh;
+          progress unfold rh)
+     end).
+
+  Local Ltac t_ext' :=
+    idtac;
+    match goal with
+      | _ => reflexivity
+      | _ => solve [ eauto with nocore ]
+      | _ => progress intros
+      | _ => progress subst
+      | [ |- @list_rect ?A ?P ?Pn ?Pc ?ls = @list_rect ?A ?P ?Pn' ?Pc' ?ls ]
+        => apply (@list_rect_ext A P Pn Pn' Pc Pc' ls)
+      | [ |- @option_rect ?A ?P ?Ps ?Pn ?x = @option_rect ?A ?P ?Ps' ?Pn' ?x ]
+        => apply (@option_rect_ext A P Ps Ps' Pn Pn' x)
+      | [ |- @List.fold_left ?A ?B _ _ _ = @List.fold_left ?A ?B _ _ _ ]
+        => let lem := constr:(_ : Proper (_ ==> _ ==> _ ==> eq) (@List.fold_left A B)) in
+           apply lem
+      | [ |- @List.fold_right ?A ?B _ _ _ = @List.fold_right ?A ?B _ _ _ ]
+        => let lem := constr:(_ : Proper (_ ==> _ ==> _ ==> eq) (@List.fold_right A B)) in
+           apply lem
+      | [ |- @List.map ?A ?B _ _ = @List.map ?A ?B _ _ ]
+        => let lem := constr:(_ : Proper (_ ==> _ ==> eq) (@List.map A B)) in
+           apply lem
+      | [ |- andb ?x _ = andb ?x _ ] => apply f_equal
+      | [ |- andb _ ?x = andb _ ?x ] => apply f_equal2
+      | _ => progress autounfold with boolr_ext_db
+      | [ |- appcontext[match ?e with _ => _ end] ] => is_var e; destruct e
+      | [ |- appcontext[match ?e with _ => _ end] ] => destruct e eqn:?
+      | [ H : _ |- _ ] => rewrite H
+      | _ => progress autorewrite with boolr_ext_db
+      | _ => progress simpl option_rect
+    end.
+
+  Local Ltac t_ext tac := repeat (t_ext' || tac).
+
+  Global Instance parse_item'_Proper
+  : Proper (pointwise_relation _ eq ==> eq ==> eq ==> eq) (parse_item').
+  Proof. t_ext expand'. Qed.
+
+  Lemma parse_item'_ext
+        (str_matches_nonterminal str_matches_nonterminal' : String.string -> bool)
+        (ext : forall s, str_matches_nonterminal s = str_matches_nonterminal' s)
+        (str : String)
+        (it : item Char)
+  : parse_item' str_matches_nonterminal str it
+    = parse_item' str_matches_nonterminal' str it.
+  Proof.
+    change ((pointwise_relation _ eq) str_matches_nonterminal str_matches_nonterminal') in ext.
+    rewrite ext; reflexivity.
+  Qed.
+
+  Hint Rewrite parse_item'_ext : boolr_ext_db.
+
+  Inductive drop_takeT := drop_of (n : nat) | take_of (n : nat).
+
+  Fixpoint drop_takes (ns : list drop_takeT) (str : String)
+    := match ns with
+         | nil => str
+         | cons (drop_of n) ns' => drop n (drop_takes ns' str)
+         | cons (take_of n) ns' => take n (drop_takes ns' str)
+       end.
+
+  Section production_drop_take.
+    Context {len0}
+            (parse_nonterminal parse_nonterminal'
+             : forall (str : String) (len : nat),
+                 len <= len0
+                 -> String.string
+                 -> bool).
+
+    Lemma parse_production'_for_ext_drop_take
+          splits splits'
+          (Hsplits : forall idx it its, splits idx it its = splits' idx it its)
+          (str : String)
+          (ext : forall ns len pf nt,
+                     @parse_nonterminal (drop_takes ns str) len pf nt
+                     = @parse_nonterminal' (drop_takes ns str) len pf nt)
+          (len : nat)
+          (pf : len <= len0)
+          (prod : production Char)
+          (ns : list _)
+    : parse_production'_for parse_nonterminal splits (drop_takes ns str) pf prod
+      = parse_production'_for parse_nonterminal' splits' (drop_takes ns str) pf prod.
+    Proof.
+      revert ns splits splits' Hsplits str ext len pf; induction prod; simpl; intros;
+      t_ext idtac.
+      erewrite parse_item'_ext.
+      { apply f_equal.
+        specialize (fun n ns => IHprod (drop_of n :: ns)%list); simpl in IHprod.
+        auto with nocore. }
+      { specialize (fun n ns => ext (take_of n :: ns)%list); simpl in ext.
+        auto with nocore. }
+    Qed.
+
+    Definition parse_production'_ext_drop_take
+               (str : String)
+               (ext : forall ns len pf nt,
+                        @parse_nonterminal (drop_takes ns str) len pf nt
+                        = @parse_nonterminal' (drop_takes ns str) len pf nt)
+               (len : nat)
+               (pf : len <= len0)
+               (prod : production Char)
+               (ns : list _)
+    : parse_production' parse_nonterminal (drop_takes ns str) pf prod
+      = parse_production' parse_nonterminal' (drop_takes ns str) pf prod
+      := parse_production'_for_ext_drop_take _ _ (fun _ _ _ => eq_refl) str ext pf prod ns.
+  End production_drop_take.
+
+  Section production.
+    Context {len0}
+            (parse_nonterminal parse_nonterminal'
+             : forall (str : String) (len : nat),
+                 len <= len0
+                 -> String.string
+                 -> bool)
+            (ext : forall str len pf nt,
+                     parse_nonterminal str len pf nt
+                     = parse_nonterminal' str len pf nt).
+
+    Lemma parse_production'_for_ext
+          splits splits'
+          (Hsplits : forall idx it its, splits idx it its = splits' idx it its)
+          (str : String)
+          (len : nat)
+          (pf : len <= len0)
+          (prod : production Char)
+    : parse_production'_for parse_nonterminal splits str pf prod
+      = parse_production'_for parse_nonterminal' splits' str pf prod.
+    Proof.
+      apply parse_production'_for_ext_drop_take with (ns := nil); auto with nocore.
+    Qed.
+
+    Definition parse_production'_ext
+               (str : String)
+               (len : nat)
+               (pf : len <= len0)
+               (prod : production Char)
+    : parse_production' parse_nonterminal str pf prod
+      = parse_production' parse_nonterminal' str pf prod
+      := parse_production'_for_ext _ _ (fun _ _ _ => eq_refl) str pf prod.
+  End production.
+
+  Global Instance parse_production'_for_Proper
+  : Proper ((pointwise_relation _ (forall_relation (fun _ => pointwise_relation _ (pointwise_relation _ eq))))
+              ==> (pointwise_relation _ (pointwise_relation _ (pointwise_relation _ eq)))
+              ==> eq
+              ==> forall_relation (fun _ => eq ==> eq ==> eq))
+           (parse_production'_for (len0 := len0)).
+  Proof.
+    repeat intro; subst.
+    apply parse_production'_for_ext;
+    assumption.
+  Qed.
+
+  Global Instance parse_production'_Proper
+  : Proper ((pointwise_relation _ (forall_relation (fun _ => pointwise_relation _ (pointwise_relation _ eq))))
+              ==> eq
+              ==> forall_relation (fun _ => eq ==> eq ==> eq))
+           (parse_production' (len0 := len0)).
+  Proof.
+    repeat intro; subst.
+    apply parse_production'_ext.
+    assumption.
+  Qed.
+
+  Section productions_drop_take.
+    Context {len0}
+            (parse_nonterminal parse_nonterminal'
+             : forall (str : String)
+                      (len : nat)
+                      (pf : len <= len0),
+                 String.string -> bool).
+
+    Lemma parse_productions'_ext_drop_take
+          (str : String)
+          (ext : forall ns str len pf nt,
+                   @parse_nonterminal (drop_takes ns str) len pf nt
+                   = @parse_nonterminal' (drop_takes ns str) len pf nt)
+          (len : nat)
+          (pf : len <= len0)
+          (prods : productions Char)
+          ns
+    : parse_productions' parse_nonterminal (drop_takes ns str) pf prods
+      = parse_productions' parse_nonterminal' (drop_takes ns str) pf prods.
+    Proof.
+      t_ext ltac:(erewrite parse_production'_for_ext_drop_take || expand').
+    Qed.
+  End productions_drop_take.
+
+  Section productions.
+    Context {len0}
+            (parse_nonterminal parse_nonterminal'
+             : forall (str : String)
+                      (len : nat)
+                      (pf : len <= len0),
+                 String.string -> bool)
+            (ext : forall str len pf nt,
+                     parse_nonterminal str len pf nt
+                     = parse_nonterminal' str len pf nt).
+
+    Lemma parse_productions'_ext
+               (str : String)
+               (len : nat)
+               (pf : len <= len0)
+               (prods : productions Char)
+    : parse_productions' parse_nonterminal str pf prods
+      = parse_productions' parse_nonterminal' str pf prods.
+    Proof.
+      apply parse_productions'_ext_drop_take with (ns := nil); auto with nocore.
+    Qed.
+  End productions.
+
+  Global Instance parse_productions'_Proper
+  : Proper ((pointwise_relation _ (forall_relation (fun _ => pointwise_relation _ (pointwise_relation _ eq))))
+              ==> eq
+              ==> forall_relation (fun _ => eq ==> eq ==> eq))
+           (parse_productions' (len0 := len0)).
+  Proof.
+    repeat intro; subst.
+    apply parse_productions'_ext.
+    assumption.
+  Qed.
+
+  Section nonterminals.
+    Section step_drop_take.
+      Context {len0 valid_len}
+              (parse_nonterminal parse_nonterminal'
+               : forall (p : nat * nat),
+                   Wf.prod_relation lt lt p (len0, valid_len)
+                   -> forall (valid : nonterminals_listT)
+                             (str : String) (len : nat),
+                        len <= fst p -> String.string -> bool).
+
+      Definition parse_nonterminal_step_ext_drop_take
+                 (valid : nonterminals_listT)
+                 (str : String)
+                 (ext : forall ns p pf valid str len pf' nt,
+                          @parse_nonterminal p pf valid (drop_takes ns str) len pf' nt
+                          = @parse_nonterminal' p pf valid (drop_takes ns str) len pf' nt)
+                 (len : nat)
+                 (pf : len <= len0)
+                 (nt : String.string)
+                 ns
+      : parse_nonterminal_step (G := G) parse_nonterminal valid (drop_takes ns str) pf nt
+        = parse_nonterminal_step (G := G) parse_nonterminal' valid (drop_takes ns str) pf nt.
+      Proof.
+        t_ext ltac:(erewrite parse_productions'_ext_drop_take || expand').
+      Qed.
+    End step_drop_take.
+
+    Section step.
+      Context {len0 valid_len}
+              (parse_nonterminal parse_nonterminal'
+               : forall (p : nat * nat),
+                   Wf.prod_relation lt lt p (len0, valid_len)
+                   -> forall (valid : nonterminals_listT)
+                             (str : String) (len : nat),
+                        len <= fst p -> String.string -> bool)
+              (ext : forall p pf valid str len pf' nt,
+                       parse_nonterminal p pf valid str len pf' nt
+                       = parse_nonterminal' p pf valid str len pf' nt).
+
+      Definition parse_nonterminal_step_ext
+                 (valid : nonterminals_listT)
+                 (str : String)
+                 (len : nat)
+                 (pf : len <= len0)
+                 (nt : String.string)
+      : parse_nonterminal_step (G := G) parse_nonterminal valid str pf nt
+        = parse_nonterminal_step (G := G) parse_nonterminal' valid str pf nt.
+      Proof.
+        apply parse_nonterminal_step_ext_drop_take with (ns := nil); auto with nocore.
+      Qed.
+    End step.
+
+    Global Instance parse_nonterminal_step_Proper
+    : Proper ((forall_relation (fun _ => pointwise_relation _ (pointwise_relation _ (pointwise_relation _ (forall_relation (fun _ => pointwise_relation _ (pointwise_relation _ eq)))))))
+                ==> eq
+                ==> eq
+                ==> forall_relation (fun _ => eq ==> eq ==> eq))
+             (parse_nonterminal_step (G := G) (len0 := len0) (valid_len := valid_len)).
+    Proof.
+      repeat intro; subst.
+      apply parse_nonterminal_step_ext.
+      assumption.
+    Qed.
+  End nonterminals.
+End recursive_descent_parser.
