src/Parsers/BooleanRecognizerOptimized.v
@@ -250,7 +250,7 @@ Section recursive_descent_parser.
            generalize (@nil take_or_drop); induction (rwf a') as [?? IH]; intros
     end.
     rewrite !Fix5_eq by (intros; apply parse_nonterminal_step_ext; assumption).
-    unfold P0' at 1, P1' at 1, parse_nonterminal_step, parse_productions', parse_production', parse_item'.
+    unfold P0' at 1, P1' at 1, parse_nonterminal_step, parse_productions', parse_production', parse_production'_for, parse_item'.
     t_reduce_fix;
     t_reduce_list;
     t_reduce_fix.
@@ -383,7 +383,7 @@ Section recursive_descent_parser.
     cbv beta iota zeta delta [parse_nonterminal parse_nonterminal_or_abort parse_nonterminal_step parse_productions parse_productions' parse_production parse_item parse_item' Lookup list_to_grammar list_to_productions].
     simpl.
     refine_Fix5_Proper_eq.
-    unfold parse_production', parse_item'.
+    unfold parse_production', parse_production'_for, parse_item'.
     fix_trans;
       [
       | solve [ t_reduce_fix;
